\documentclass{amsart}
\usepackage{graphicx}
\usepackage{fancyhdr}
\usepackage{verbatim}
\usepackage{bm}
\usepackage[colorlinks=true, urlcolor=blue, citecolor=blue, linkcolor=blue, book
marks=true, ]{hyperref}
\usepackage[top=3cm,right=3cm,left=3cm]{geometry}

\DeclareMathOperator{\erf}{erf}
\newcommand{\D}[2]{\ensuremath{\frac{d{#1}}{d{#2}}}}
\newcommand{\Dp}[2]{\ensuremath{\frac{\partial{#1}}{\partial{#2}}}}

\begin{document}

\section{Definitions}

\begin{itemize}
\item $x$: weighted pixel vector
\item $\Sigma$: pixel covariance matrix (assumed to be diagonal)
\item $\phi$: nonlinear parameters
\item $\alpha$: flux coefficients
\item $\mu$: morphology parameters
\item $y(\phi)$: morphology prior mean
\item $F(\phi)$: morphology prior Fisher matrix
\item $M(\phi)$: morphology model matrix
\item $A(\phi)$: flux model matrix
\item $s(\phi,\alpha,\mu) = (M\mu + A\alpha - x)$: residual vector
\end{itemize}

\section{Bayesian Probabilities}

\begin{eqnarray}
  P(\phi,\alpha,\mu|x) &=& P(x|\phi,\alpha,\mu)
  \frac{P(\phi,\alpha,\mu)}{P(x)} \\
  P(\phi,\alpha|x)P(\mu|x,\phi,\alpha) &=&
  P(x|\phi,\alpha,\mu)\frac{P(\mu|\phi,\alpha) P(\phi,\alpha)}{P(x)}
  \\
  P(\phi,\alpha|x) &=& \frac{P(\phi,\alpha)}{P(x)}
  \int d\mu P(\mu|\phi,\alpha) P(x|\phi,\alpha,\mu) \\
  &=& \frac{P(\phi,\alpha)}{P(x)} P(x|\phi,\alpha)
\end{eqnarray}

\section{Morphology Marginalization}

($\phi$ dependence implicit in $A$, $M$, $F$, $y$, $s$)

\begin{eqnarray}
  q(\alpha,\mu) &\equiv& -\ln P(x|\phi,\alpha,\mu) 
  - \ln P(\mu|\alpha) \\ &=& 
  \frac{1}{2}||s(\alpha,\mu)||^2
  + \frac{1}{2} \left(\mu - y\right)^T\! 
  F \left(\mu - y\right) \\
  & & + \frac{1}{2}\ln\left|2\pi\Sigma\right|
  + \frac{1}{2}\ln\left|2\pi F^{-1}\right| \\
  \Dp{q}{\mu} &=& M^T\!s(\alpha,\mu) + F \left(\mu - y\right) \\
  \Dp{^2q}{\mu^2} &=& M^T\!M + F \\
  \Dp{q}{\alpha} &=& A^T\!s(\alpha,\mu) \\
  \Dp{^2q}{\alpha^2} &=& A^T\!A \\
  \Dp{^2q}{\alpha\partial\mu} &=& M^T\!A 
\end{eqnarray}

\begin{eqnarray}
  \hat{\mu}(\alpha) &=& \left(M^T\!M + F\right)^{-1}
  \left(M^T\!x - M^T\!A\alpha+ Fy\right) \\
  &=& H^{-1} \left(M^T\!x - M^T\!A\alpha + Fy\right) \\
  &=& b + B\alpha \\
  B &\equiv& \Dp{\hat{\mu}}{\alpha} =  -H^{-1}M^T\!A \\
  b &\equiv& H^{-1}\left(M^T\!x + Fy\right)
\end{eqnarray}

\begin{equation}
  q(\alpha,\mu) = q(\alpha,\hat{\mu}(\alpha)) +
  \frac{1}{2}\left[\mu-\hat{\mu}(\alpha)\right]^T\!\left[M^T\!M + F\right]
  \left[\mu-\hat{\mu}(\alpha)\right]
\end{equation}

\begin{eqnarray}
  p(\alpha) &\equiv& -\ln\int_{K\mu > c}\!\!\!\!\!\!\!\!
  e^{-q(\alpha,\mu)} d\mu \\
  &=& -\ln P(x|\phi,\alpha) \\
    &=& q(\alpha,\hat{\mu}(\alpha)) 
  + \frac{1}{2}\ln\left|\frac{M^T\!M + F}{2\pi}\right|
  - \ln r(\alpha)
\end{eqnarray}

where $r(\alpha)$ is the fraction of Monte Carlo samples drawn from a
Gaussian with mean $\hat{\mu}$ and covariance $(M^T\!M + F)^{-1}$ that
obey the inequality constraint $K\mu > c$.

\begin{eqnarray}
  \D{[q(\alpha,\hat{\mu}(\alpha))]}{\alpha} &=& \Dp{q}{\alpha} +
  \Dp{\hat{\mu}}{\alpha}\Dp{q}{\mu} \\
  &=& A^T\!s(\alpha,\hat{\mu}(\alpha)) 
  + B^T M^Ts(\alpha,\hat{\mu}(\alpha)) \\
  &=& \left(A + M B \right)^T s(\alpha,\hat{\mu}(\alpha)) \\
  &=& \left(A + M B \right)^T \left(A\alpha + Mb + M B \alpha -
  x\right) \\
  &=& \left(A + M B \right)^T \left[\left(A + M B\right)\alpha + Mb -
    x\right] \\
  &=& (A+MB)^T\!(A+MB)\alpha + (A + MB)^T\!(Mb - x)\\
  \D{^2[q(\alpha,\hat{\mu}(\alpha))]}{\alpha^2} &=& (A+MB)^T\!(A+MB) \equiv G
\end{eqnarray}

\begin{equation}
  \hat{\alpha} = G^{-1}\!(A + MB)^T\!(x - Mb)
\end{equation}

\begin{eqnarray}
  p(\alpha) = q(\hat{\alpha},\hat{\mu}(\hat{\alpha}))
  + \frac{1}{2}\ln\left|\frac{M^T\!M + F}{2\pi}\right|
  + \frac{1}{2}\left(\alpha - \hat{\alpha}\right)^T\!
  G \left(\alpha - \hat{\alpha}\right)
  - \ln r(\alpha)
\end{eqnarray}

\end{document}
